eval/scripts/tabulate-missing-ops.sh
@@ -1,0 +1,13 @@
+#!/bin/bash
+set -euo pipefail
+shopt -s nullglob
+
+scripts_dir="$(cd -- "$(dirname -- "${BASH_SOURCE[0]}")" &> /dev/null && pwd)"
+source "${scripts_dir}/common.sh"
+
+grep -REoh 'undefined op `([^`]+)`' "${failed_compile_logs_dir}" \
+  | sed 's,undefined op ,,' \
+  | sed 's,`,,g' \
+  | sort \
+  | uniq -c \
+  | sort -hr
