scripts/verify.sh
@@ -6,6 +6,6 @@ shift
 
 repo_dir="$(cd -- "$(dirname -- "${BASH_SOURCE[0]}")" &> /dev/null && cd .. && pwd)"
 bpl_file="${repo_dir}/out/${sample_name}.bpl"
-corral_exe="${repo_dir}/vendor/corral/source/Corral/bin/Release/net5.0/corral"
+corral_exe="${repo_dir}/vendor/corral/source/Corral/bin/Release/net6.0/corral"
 
 "${corral_exe}" "${bpl_file}" /trackAllVars /recursionBound:4 "${@}"
